ironfleet/src/Dafny/Distributed/Concur/Movers.i.dfy
@@ -24,80 +24,79 @@ module MoversModule {
         ActionIsLeftMover(entry.action)
     }
 
-
     lemma lemma_MoverCommutativityForEntries(
         entry1:Entry,
         entry2:Entry,
-        ds1:SystemState,
-        ds2:SystemState,
-        ds3:SystemState
+        ls1:SystemState,
+        ls2:SystemState,
+        ls3:SystemState
         )
         returns
-        (ds2':SystemState)
+        (ls2':SystemState)
         requires entry1.actor != entry2.actor;
-        requires SystemNextEntry(ds1, ds2, entry1);
-        requires SystemNextEntry(ds2, ds3, entry2);
+        requires SystemNextEntry(ls1, ls2, entry1);
+        requires SystemNextEntry(ls2, ls3, entry2);
         requires EntryIsRightMover(entry1) || EntryIsLeftMover(entry2);
-        ensures  SystemNextEntry(ds1, ds2', entry2);
-        ensures  SystemNextEntry(ds2', ds3, entry1);
+        ensures  SystemNextEntry(ls1, ls2', entry2);
+        ensures  SystemNextEntry(ls2', ls3, entry1);
     {
         if entry1.action.Receive? {
-            ds2' := ds3;
+            ls2' := ls3;
         }
         else if entry1.action.UpdateLocalState? {
-            if entry1.actor in ds1.states {
-                ds2' := ds3.(states := ds3.states[entry1.actor := ds1.states[entry1.actor]]);
+            if entry1.actor in ls1.states {
+                ls2' := ls3.(states := ls3.states[entry1.actor := ls1.states[entry1.actor]]);
                 if !entry2.action.UpdateLocalState? && !entry2.action.PerformIos? && !entry2.action.HostNext? {
-                    assert ds2'.states == ds1.states;
+                    assert ls2'.states == ls1.states;
                 }
             }
-            else if entry1.actor in ds2.states {
-                ds2' := ds3.(states := mapremove(ds3.states, entry1.actor));
+            else if entry1.actor in ls2.states {
+                ls2' := ls3.(states := mapremove(ls3.states, entry1.actor));
                 if !entry2.action.UpdateLocalState? && !entry2.action.PerformIos? && !entry2.action.HostNext? {
-                    assert ds2'.states == ds1.states;
+                    assert ls2'.states == ls1.states;
                 }
             }
             else {
-                assert ds1.states == ds2.states;
-                ds2' := ds3;
+                assert ls1.states == ls2.states;
+                ls2' := ls3;
             }
         }
         else if entry2.action.UpdateLocalState? {
-            if entry2.actor in ds2.states {
-                if entry2.actor in ds3.states {
-                    ds2' := ds1.(states := ds1.states[entry2.actor := ds3.states[entry2.actor]]);
+            if entry2.actor in ls2.states {
+                if entry2.actor in ls3.states {
+                    ls2' := ls1.(states := ls1.states[entry2.actor := ls3.states[entry2.actor]]);
                 }
                 else {
-                    ds2' := ds1.(states := mapremove(ds1.states, entry2.actor));
+                    ls2' := ls1.(states := mapremove(ls1.states, entry2.actor));
                 }
                 if !entry1.action.UpdateLocalState? && !entry1.action.PerformIos? && !entry1.action.HostNext? {
-                    assert ds2'.states == ds3.states;
+                    assert ls2'.states == ls3.states;
                 }
             }
             else {
-                if entry2.actor in ds3.states {
-                    ds2' := ds1.(states := ds1.states[entry2.actor := ds3.states[entry2.actor]]);
+                if entry2.actor in ls3.states {
+                    ls2' := ls1.(states := ls1.states[entry2.actor := ls3.states[entry2.actor]]);
                     if !entry1.action.UpdateLocalState? && !entry1.action.PerformIos? && !entry1.action.HostNext? {
-                        assert ds2'.states == ds3.states;
+                        assert ls2'.states == ls3.states;
                     }
                 }
                 else {
-                    ds2' := ds1;
-                    assert ds2.states == ds3.states;
+                    ls2' := ls1;
+                    assert ls2.states == ls3.states;
                 }
             }
         }
         else if entry2.action.Send? {
-            ds2' := ds1.(sentPackets := ds1.sentPackets + {entry2.action.s});
+            ls2' := ls1.(sentPackets := ls1.sentPackets + {entry2.action.s});
             if entry1.action.Send? {
-                assert ds2'.states == ds3.states;
-                assert ds3.sentPackets == ds2'.sentPackets + {entry1.action.s};
+                assert ls2'.states == ls3.states;
+                assert ls3.sentPackets == ls2'.sentPackets + {entry1.action.s};
             }
             else if entry1.action.PerformIos? {
-                assert ds2'.states == ds1.states;
+                assert ls2'.states == ls1.states;
             }
             else if entry1.action.HostNext? {
-                assert ds2'.states == ds1.states;
+                assert ls2'.states == ls1.states;
             }
         }
     }
